feat(Languages/LambdaCalculus/LocallyNameless): Fsub (#68)
* cleaning, docs

* map_subst

* rest of porting

* rm weaken_head TODO

* easy parts of preservation

* some docs

* more preservation

* finish preservation

* all but trans case of map_subst

* easy weaken cases

* half of the trans case

* complete map_subst

* type weakening

* narrow

* style

* donegit st!

* rm duplicated API

* redundant lemma

* large union trouble

* old TODOs

* style

* prefer Type*

* docs typo

* golfing

* naming convention, unused hypothesis

* better proof of keys_append

* redundant keys lemma

* a few more unused context lemmas

* style

* better sublist_dlookup proof

* better generality for nodupKeys_middle

Cslib/Languages/LambdaCalculus/LocallyNameless/Context.lean
@@ -17,43 +17,96 @@ Contexts as pairs of free variables and types.
 
 universe u v
 
-variable {Var : Type u} {Ty : Type v} [DecidableEq Var]
+variable {α : Type u} {β : Type v}
+
+-- TODO: These are pieces of API that cannot be directly automated by adding `grind` attributes to
+-- `Mathlib.Data.List.Sigma`. We should consider upstreaming them to Mathlib.
+namespace List
+
+variable {β : α → Type v} {l₁ l₂ : List (Sigma β)}
+
+/-- Keys distribute with appending. -/
+theorem keys_append : (l₁ ++ l₂).keys = l₁.keys ++ l₂.keys := by
+  simp [keys]
+
+variable [DecidableEq α] in
+/-- Sublists without duplicate keys preserve lookups. -/
+theorem sublist_dlookup (nd₂ : l₂.NodupKeys) (s : l₁ <+ l₂) (mem : b ∈ l₁.dlookup a) : 
+    b ∈ l₂.dlookup a := by
+  grind [Option.mem_def, → perm_nodupKeys, dlookup_append, => perm_dlookup,
+    → Sublist.exists_perm_append]
+
+@[grind =]
+lemma nodupKeys_middle : (l₁ ++ s :: l₂).NodupKeys ↔ (s :: (l₁ ++ l₂)).NodupKeys := by
+  simp_all [NodupKeys, keys, nodup_middle]
+
+end List
 
 namespace LambdaCalculus.LocallyNameless
 
+variable [DecidableEq α]
+
 /-- A typing context is a list of free variables and corresponding types. -/
-abbrev Context (Var : Type u) (Ty : Type v) := List ((_ : Var) × Ty)
+abbrev Context (α : Type u) (β : Type v) := List ((_ : α) × β)
 
 namespace Context
 
 open List
 
+-- we would like grind to see through certain notations
+attribute [scoped grind =] Option.mem_def
+attribute [scoped grind _=_] List.append_eq
+attribute [scoped grind =] List.Nodup
+attribute [scoped grind =] List.NodupKeys
+attribute [scoped grind _=_] List.singleton_append
+
+-- a few grinds on Option:
+attribute [scoped grind =] Option.or_eq_some_iff
+attribute [scoped grind =] Option.or_eq_none_iff
+
+-- we would like grind to treat list and finset membership the same
+attribute [scoped grind _=_] List.mem_toFinset
+
+-- otherwise, we mostly reuse existing API in `Mathlib.Data.List.Sigma`
+attribute [scoped grind =] List.keys_cons
+attribute [scoped grind =] List.dlookup_cons_eq
+attribute [scoped grind =] List.dlookup_cons_ne
+attribute [scoped grind =] List.dlookup_nil
+attribute [scoped grind _=_] List.dlookup_isSome
+attribute [scoped grind →] List.perm_nodupKeys
+
 /-- The domain of a context is the finite set of free variables it uses. -/
 @[simp, grind =]
-def dom : Context Var Ty → Finset Var := toFinset ∘ keys
+def dom (Γ : Context α β) : Finset α := Γ.keys.toFinset
 
-/-- A well-formed context. -/
-abbrev Ok : Context Var Ty → Prop := NodupKeys
+instance : HasWellFormed (Context α β) :=
+  ⟨NodupKeys⟩
 
-instance : HasWellFormed (Context Var Ty) :=
-  ⟨Ok⟩
+omit [DecidableEq α] in
+@[scoped grind _=_]
+theorem haswellformed_def (Γ : Context α β) : Γ✓ = Γ.NodupKeys := by rfl
 
-variable {Γ Δ : Context Var Ty}
+variable {Γ Δ : Context α β}
 
-/-- Context membership is preserved on permuting a context. -/
-theorem dom_perm_mem_iff (h : Γ.Perm Δ) {x : Var} : x ∈ Γ.dom ↔ x ∈ Δ.dom := by
-  induction h <;> simp_all only [dom, Function.comp_apply, mem_toFinset, keys_cons, mem_cons] 
-  grind
-
-omit [DecidableEq Var] in
-/-- Context well-formedness is preserved on permuting a context. -/
-@[scoped grind →]
-theorem wf_perm (h : Γ.Perm Δ) : Γ✓ → Δ✓ := (List.perm_nodupKeys h).mp
-
-omit [DecidableEq Var] in
+omit [DecidableEq α] in
 /-- Context well-formedness is preserved on removing an element. -/
 @[scoped grind →]
 theorem wf_strengthen (ok : (Δ ++ ⟨x, σ⟩ :: Γ)✓) : (Δ ++ Γ)✓ := by
-  exact List.NodupKeys.sublist (by simp) ok
+  grind [keys_append]
+
+/-- A mapping of values within a context. -/
+@[simp, scoped grind]
+def map_val (f : β → β) (Γ : Context α β) : Context α β := 
+  Γ.map (fun ⟨var,ty⟩ => ⟨var,f ty⟩)
+
+omit [DecidableEq α] in
+/-- A mapping of values preserves keys. -/
+@[scoped grind]
+lemma map_val_keys (f) : Γ.keys = (Γ.map_val f).keys := by
+  induction Γ <;> grind
+
+/-- A mapping of values maps lookups. -/
+lemma map_val_mem (mem : σ ∈ Γ.dlookup x) (f) : f σ ∈ (Γ.map_val f).dlookup x := by
+  induction Γ <;> grind
 
 end LambdaCalculus.LocallyNameless.Context
