Cslib/Languages/LambdaCalculus/LocallyNameless/Fsub/Basic.lean
@@ -1,0 +1,107 @@
+/-
+Copyright (c) 2025 Chris Henson. All rights reserved.
+Released under Apache 2.0 license as described in the file LICENSE.
+Authors: Chris Henson
+-/
+
+import Cslib.Foundations.Data.HasFresh
+import Cslib.Foundations.Syntax.HasSubstitution
+import Cslib.Languages.LambdaCalculus.LocallyNameless.Context
+
+/-! # λ-calculus
+
+The λ-calculus with polymorphism and subtyping, with a locally nameless representation of syntax.
+
+## References
+
+* [A. Chargueraud, *The Locally Nameless Representation*][Chargueraud2012]
+* See also <https://www.cis.upenn.edu/~plclub/popl08-tutorial/code/>, from which
+  this is adapted
+
+-/
+
+variable {Var : Type*} [HasFresh Var] [DecidableEq Var]
+
+namespace LambdaCalculus.LocallyNameless.Fsub
+
+/-- Types of the polymorphic lambda calculus. -/
+inductive Ty (Var : Type*)
+  /-- The type ⊤, with a single inhabitant. -/
+  | top : Ty Var
+  /-- Bound variables that appear in a type, using a de-Bruijn index. -/
+  | bvar : ℕ → Ty Var
+  /-- Free type variables. -/
+  | fvar : Var → Ty Var
+  /-- A function type. -/
+  | arrow : Ty Var → Ty Var → Ty Var
+  /-- A universal quantification. -/
+  | all : Ty Var → Ty Var → Ty Var
+  /-- A sum type. -/
+  | sum : Ty Var → Ty Var → Ty Var
+  deriving Inhabited
+
+/-- Syntax of locally nameless lambda terms, with free variables over `Var`. -/
+inductive Term (Var : Type*)
+  /-- Bound term variables that appear under a lambda abstraction, using a de-Bruijn index. -/
+  | bvar : ℕ → Term Var
+  /-- Free term variables. -/
+  | fvar : Var → Term Var
+  /-- Lambda abstraction, introducing a new bound term variable. -/
+  | abs : Ty Var → Term Var → Term Var
+  /-- Function application. -/
+  | app : Term Var → Term Var → Term Var
+  /-- Type abstraction, introducing a new bound type variable. -/
+  | tabs : Ty Var → Term Var → Term Var
+  /-- Type application. -/
+  | tapp : Term Var → Ty Var → Term Var
+  /-- Binding of a term. -/
+  | let' : Term Var → Term Var → Term Var
+  /-- Left constructor of a sum. -/
+  | inl : Term Var → Term Var
+  /-- Right constructor of a sum. -/
+  | inr : Term Var → Term Var
+  /-- Case matching on a sum. -/
+  | case : Term Var → Term Var → Term Var → Term Var
+
+/-- A context binding. -/
+inductive Binding (Var : Type*)
+  /-- Subtype binding. -/
+  | sub : Ty Var → Binding Var
+  /-- Type binding. -/
+  | ty : Ty Var → Binding Var
+  deriving Inhabited
+
+/-- Free variables of a type. -/
+@[scoped grind =]
+def Ty.fv : Ty Var → Finset Var
+| top | bvar _ => {}
+| fvar X => {X}
+| arrow σ τ | all σ τ | sum σ τ => σ.fv ∪ τ.fv
+
+/-- Free variables of a binding. -/
+@[scoped grind =]
+def Binding.fv : Binding Var → Finset Var
+| sub σ | ty σ => σ.fv
+
+/-- Free type variables of a term. -/
+@[scoped grind =]
+def Term.fv_ty : Term Var → Finset Var
+| bvar _ | fvar _ => {}
+| abs σ t₁ | tabs σ t₁ | tapp t₁ σ => σ.fv ∪ t₁.fv_ty
+| inl t₁ | inr t₁ => t₁.fv_ty
+| app t₁ t₂ | let' t₁ t₂ => t₁.fv_ty ∪ t₂.fv_ty
+| case t₁ t₂ t₃ => t₁.fv_ty ∪ t₂.fv_ty ∪ t₃.fv_ty
+
+/-- Free term variables of a term. -/
+@[scoped grind =]
+def Term.fv_tm : Term Var → Finset Var
+| bvar _ => {}
+| fvar x => {x}
+| abs _ t₁ | tabs _ t₁ | tapp t₁ _ | inl t₁ | inr t₁ => t₁.fv_tm
+| app t₁ t₂ | let' t₁ t₂ => t₁.fv_tm ∪ t₂.fv_tm
+| case t₁ t₂ t₃ => t₁.fv_tm ∪ t₂.fv_tm ∪ t₃.fv_tm
+
+/-- A context of bindings. -/
+abbrev Env (Var : Type*) := Context Var (Binding Var)
+
+end LambdaCalculus.LocallyNameless.Fsub
