Cslib/Languages/LambdaCalculus/LocallyNameless/Fsub/Opening.lean
@@ -1,0 +1,416 @@
+/-
+Copyright (c) 2025 Chris Henson. All rights reserved.
+Released under Apache 2.0 license as described in the file LICENSE.
+Authors: Chris Henson
+-/
+
+import Cslib.Languages.LambdaCalculus.LocallyNameless.Fsub.Basic
+
+
+/-! # λ-calculus
+
+The λ-calculus with polymorphism and subtyping, with a locally nameless representation of syntax.
+This file defines opening, local closure, and substitution.
+
+## References
+
+* [A. Chargueraud, *The Locally Nameless Representation*][Chargueraud2012]
+* See also <https://www.cis.upenn.edu/~plclub/popl08-tutorial/code/>, from which
+  this is adapted
+
+-/
+
+variable {Var : Type*} [HasFresh Var] [DecidableEq Var]
+
+namespace LambdaCalculus.LocallyNameless.Fsub
+
+namespace Ty
+
+/-- Variable opening (type opening to type) of the ith bound variable. -/
+@[scoped grind =]
+def openRec (X : ℕ) (δ : Ty Var) : Ty Var → Ty Var
+| top => top
+| bvar Y => if X = Y then δ else bvar Y
+| fvar X => fvar X
+| arrow σ τ => arrow (openRec X δ σ) (openRec X δ τ)
+| all σ τ => all (openRec X δ σ) (openRec (X + 1) δ τ)
+| sum σ τ => sum (openRec X δ σ) (openRec X δ τ)
+
+scoped notation:68 γ "⟦" X " ↝ " δ "⟧ᵞ"=> openRec X δ γ
+
+/-- Variable opening (type opening to type) of the closest binding. -/
+@[scoped grind =]
+def open' (γ δ : Ty Var) := openRec 0 δ γ
+
+scoped infixr:80 " ^ᵞ " => open'
+
+/-- Locally closed types. -/
+inductive LC : Ty Var → Prop
+  | top : LC top
+  | var : LC (fvar X)
+  | arrow : LC σ → LC τ → LC (arrow σ τ)
+  | all (L : Finset Var) : LC σ → (∀ X ∉ L, LC (τ ^ᵞ fvar X)) → LC (all σ τ)
+  | sum : LC σ → LC τ → LC (sum σ τ)
+
+attribute [scoped grind] LC.top LC.var LC.arrow LC.sum
+
+/-- Type substitution. -/
+@[scoped grind =]
+def subst (X : Var) (δ : Ty Var) : Ty Var → Ty Var
+| top => top
+| bvar J => bvar J
+| fvar Y => if Y = X then δ else fvar Y
+| arrow σ τ => arrow (subst X δ σ) (subst X δ τ)
+| all σ τ => all (subst X δ σ) (subst X δ τ)
+| sum σ τ => sum (subst X δ σ) (subst X δ τ)
+
+instance : HasSubstitution (Ty Var) Var (Ty Var) where
+  subst γ X δ := Ty.subst X δ γ
+
+variable {σ τ δ γ : Ty Var}
+
+omit [HasFresh Var] [DecidableEq Var] in
+/-- An opening appearing in both sides of an equality of types can be removed. -/
+lemma openRec_neq_eq {σ τ γ : Ty Var} (neq : X ≠ Y) (h : σ⟦Y ↝ τ⟧ᵞ = σ⟦Y ↝ τ⟧ᵞ⟦X ↝ γ⟧ᵞ) : 
+    σ = σ⟦X ↝ γ⟧ᵞ := by induction σ generalizing Y X <;> grind
+
+/-- A locally closed type is unchanged by opening. -/
+lemma openRec_lc {σ τ : Ty Var} (lc : σ.LC) : σ = σ⟦X ↝ τ⟧ᵞ := by
+  induction lc generalizing X <;> (have := fresh_exists <| free_union Var; grind [openRec_neq_eq])
+
+omit [HasFresh Var] in
+@[scoped grind _=_]
+lemma subst_def : Ty.subst (X : Var) (δ : Ty Var) (γ : Ty Var) = γ[X := δ] := by rfl
+
+omit [HasFresh Var] in
+/-- Substitution of a free variable not present in a type leaves it unchanged. -/
+lemma subst_fresh (nmem : X ∉ γ.fv) (δ : Ty Var) : γ = γ[X := δ] := by
+  induction γ <;> grind
+
+/-- Substitution of a locally closed type distributes with opening. -/
+lemma openRec_subst (Y : ℕ) (σ τ : Ty Var) (lc : δ.LC) (X : Var) : 
+    (σ⟦Y ↝ τ⟧ᵞ)[X := δ] = σ[X := δ]⟦Y ↝ τ[X := δ]⟧ᵞ := by
+  induction σ generalizing Y
+  all_goals grind [openRec_lc]
+
+/-- Specialize `Ty.openRec_subst` to the first opening. -/
+lemma open_subst (σ τ : Ty Var) (lc : δ.LC) (X : Var) : (σ ^ᵞ τ)[X := δ] = σ[X := δ] ^ᵞ τ[X := δ]
+  := openRec_subst 0 σ τ lc X
+
+/-- Specialize `Ty.subst_open` to free variables. -/
+lemma open_subst_var (σ : Ty Var) (neq : Y ≠ X) (lc : δ.LC) :
+    (σ ^ᵞ fvar Y)[X := δ] = (σ[X := δ]) ^ᵞ fvar Y := by grind [open_subst]
+
+omit [HasFresh Var] in
+/-- Opening to a type is equivalent to opening to a free variable and substituting. -/
+lemma openRec_subst_intro (Y : ℕ) (δ : Ty Var) (nmem : X ∉ γ.fv) :
+    γ⟦Y ↝ δ⟧ᵞ = (γ⟦Y ↝ fvar X⟧ᵞ)[X := δ] := by
+  induction γ generalizing δ Y <;> grind
+
+omit [HasFresh Var] in
+/-- Specialize `Ty.openRec_subst_intro` to the first opening. -/
+lemma open_subst_intro (δ : Ty Var) (nmem : X ∉ γ.fv) : γ ^ᵞ δ = (γ ^ᵞ fvar X)[X := δ] := 
+  openRec_subst_intro _ _ nmem
+
+lemma subst_lc (σ_lc : σ.LC) (τ_lc : τ.LC) (X : Var) : σ[X := τ].LC := by
+  induction σ_lc
+  case all => apply LC.all (free_union Var) <;> grind [openRec_subst] 
+  all_goals grind [openRec_subst]
+
+omit [HasFresh Var] in
+lemma nmem_fv_openRec (nmem : X ∉ (σ⟦k ↝ γ⟧ᵞ).fv) : X ∉ σ.fv := by
+  induction σ generalizing k <;> grind
+
+omit [HasFresh Var] in
+lemma nmem_fv_open (nmem : X ∉ (σ ^ᵞ γ).fv) : X ∉ σ.fv := 
+  Ty.nmem_fv_openRec (k := 0) nmem
+
+end Ty
+
+namespace Term
+
+open scoped Ty
+
+/-- Variable opening (term opening to type) of the ith bound variable. -/
+@[scoped grind =]
+def openRec_ty (X : ℕ) (δ : Ty Var) : Term Var → Term Var
+| bvar x => bvar x
+| fvar x => fvar x
+| abs σ t₁ => abs (σ⟦X ↝ δ⟧ᵞ) (openRec_ty X δ t₁)
+| app t₁ t₂ => app (openRec_ty X δ t₁) (openRec_ty X δ t₂)
+| tabs σ t₁ => tabs (σ⟦X ↝ δ⟧ᵞ) (openRec_ty (X + 1) δ t₁)
+| tapp t₁ σ => tapp (openRec_ty X δ t₁) (σ⟦X ↝ δ⟧ᵞ)
+| let' t₁ t₂ => let' (openRec_ty X δ t₁) (openRec_ty X δ t₂)
+| inl t₁ => inl (openRec_ty X δ t₁)
+| inr t₂ => inr (openRec_ty X δ t₂)
+| case t₁ t₂ t₃ => case (openRec_ty X δ t₁) (openRec_ty X δ t₂) (openRec_ty X δ t₃)
+
+scoped notation:68 t "⟦" X " ↝ " δ "⟧ᵗᵞ"=> openRec_ty X δ t
+
+/-- Variable opening (term opening to type) of the closest binding. -/
+@[scoped grind =]
+def open_ty (t : Term Var) (δ : Ty Var) := openRec_ty 0 δ t
+
+scoped infixr:80 " ^ᵗᵞ " => open_ty
+
+/-- Variable opening (term opening to term) of the ith bound variable. -/
+@[scoped grind =]
+def openRec_tm (x : ℕ) (s : Term Var) : Term Var → Term Var
+| bvar y => if x = y then s else (bvar y)
+| fvar x => fvar x
+| abs σ t₁ => abs σ (openRec_tm (x + 1) s t₁)
+| app t₁ t₂ => app (openRec_tm x s t₁) (openRec_tm x s t₂)
+| tabs σ t₁ => tabs σ (openRec_tm x s t₁)
+| tapp t₁ σ => tapp (openRec_tm x s t₁) σ
+| let' t₁ t₂ => let' (openRec_tm x s t₁) (openRec_tm (x + 1) s t₂)
+| inl t₁ => inl (openRec_tm x s t₁)
+| inr t₂ => inr (openRec_tm x s t₂)
+| case t₁ t₂ t₃ => case (openRec_tm x s t₁) (openRec_tm (x + 1) s t₂) (openRec_tm (x + 1) s t₃)
+
+scoped notation:68 t "⟦" x " ↝ " s "⟧ᵗᵗ"=> openRec_tm x s t
+
+/-- Variable opening (term opening to term) of the closest binding. -/
+@[scoped grind =]
+def open_tm (t₁ t₂ : Term Var) := openRec_tm 0 t₂ t₁
+
+scoped infixr:80 " ^ᵗᵗ " => open_tm
+
+/-- Locally closed terms. -/
+inductive LC : Term Var → Prop
+  | var : LC (fvar x)
+  | abs (L : Finset Var) : σ.LC → (∀ x ∉ L, LC (t₁ ^ᵗᵗ fvar x)) → LC (abs σ t₁)
+  | app : LC t₁ → LC t₂ → LC (app t₁ t₂)
+  | tabs (L : Finset Var) : σ.LC → (∀ X ∉ L, LC (t₁ ^ᵗᵞ .fvar X)) → LC (tabs σ t₁)
+  | tapp : LC t₁ → σ.LC → LC (tapp t₁ σ)
+  | let' (L : Finset Var) : LC t₁ → (∀ x ∉ L, LC (t₂ ^ᵗᵗ fvar x)) → LC (let' t₁ t₂)
+  | inl : LC t₁ → LC (inl t₁)
+  | inr : LC t₁ → LC (inr t₁)
+  | case (L : Finset Var) :
+      LC t₁ →
+      (∀ x ∉ L, LC (t₂ ^ᵗᵗ fvar x)) →
+      (∀ x ∉ L, LC (t₃ ^ᵗᵗ fvar x)) →
+      LC (case t₁ t₂ t₃)
+
+attribute [scoped grind] LC.var LC.app LC.inl LC.inr LC.tapp
+
+variable {t : Term Var} {δ : Ty Var}
+
+omit [HasFresh Var] [DecidableEq Var] in
+/-- An opening (term to type) appearing in both sides of an equality of terms can be removed. -/
+lemma openRec_ty_neq_eq (neq : X ≠ Y) (eq : t⟦Y ↝ σ⟧ᵗᵞ = t⟦Y ↝ σ⟧ᵗᵞ⟦X ↝ τ⟧ᵗᵞ) : 
+    t = t⟦X ↝ τ⟧ᵗᵞ := by
+  induction t generalizing X Y <;> grind [Ty.openRec_neq_eq]
+
+omit [HasFresh Var] [DecidableEq Var] in
+/-- Elimination of mixed term and type opening. -/
+@[scoped grind]
+lemma openRec_tm_ty_eq (eq : t⟦x ↝ s⟧ᵗᵗ = t⟦x ↝ s⟧ᵗᵗ⟦y ↝ δ⟧ᵗᵞ) : t = t⟦y ↝ δ⟧ᵗᵞ
+  := by induction t generalizing x y <;> grind
+
+/-- A locally closed term is unchanged by type opening. -/
+@[scoped grind]
+lemma openRec_ty_lc {t : Term Var} (lc : t.LC) : t = t⟦X ↝ σ⟧ᵗᵞ := by
+  induction lc generalizing X
+  case let' | case | tabs | abs =>
+    have := fresh_exists <| free_union Var
+    congr <;> grind [Ty.openRec_lc, openRec_ty_neq_eq]
+  all_goals grind [Ty.openRec_lc]
+
+/-- Substitution of a type within a term. -/
+@[scoped grind =]
+def subst_ty (X : Var) (δ : Ty Var) : Term Var → Term Var
+| bvar x => bvar x
+| fvar x => fvar x
+| abs σ t₁ => abs (σ [X := δ]) (subst_ty X δ t₁)
+| app t₁ t₂ => app (subst_ty X δ t₁) (subst_ty X δ t₂)
+| tabs σ t₁ => tabs (σ [X := δ]) (subst_ty X δ t₁)
+| tapp t₁ σ => tapp (subst_ty X δ t₁) (σ[X := δ])
+| let' t₁ t₂ => let' (subst_ty X δ t₁) (subst_ty X δ t₂)
+| inl t₁ => inl (subst_ty X δ t₁)
+| inr t₁ => inr (subst_ty X δ t₁)
+| case t₁ t₂ t₃ => case (subst_ty X δ t₁) (subst_ty X δ t₂) (subst_ty X δ t₃)
+
+instance : HasSubstitution (Term Var) Var (Ty Var) where
+  subst t X δ := Term.subst_ty X δ t
+
+omit [HasFresh Var] in
+@[scoped grind _=_]
+lemma subst_ty_def : subst_ty (X : Var) (δ : Ty Var) (t : Term Var) = t[X := δ] := by rfl
+
+omit [HasFresh Var] in
+/-- Substitution of a free type variable not present in a term leaves it unchanged. -/
+lemma subst_ty_fresh (nmem : X ∉ t.fv_ty) (δ : Ty Var) : t = t [X := δ] := 
+  by induction t <;> grind [Ty.subst_fresh]
+
+/-- Substitution of a locally closed type distributes with term opening to a type . -/
+lemma openRec_ty_subst_ty (Y : ℕ) (t : Term Var) (σ : Ty Var) (lc : δ.LC) (X : Var) : 
+    (t⟦Y ↝ σ⟧ᵗᵞ)[X := δ] = (t[X := δ])⟦Y ↝  σ[X := δ]⟧ᵗᵞ := by
+  induction t generalizing Y <;> grind [Ty.openRec_subst]
+
+/-- Specialize `Term.openRec_ty_subst` to the first opening. -/
+lemma open_ty_subst_ty (t : Term Var) (σ : Ty Var) (lc : δ.LC) (X : Var) :
+     (t ^ᵗᵞ σ)[X := δ] = t[X := δ] ^ᵗᵞ σ[X := δ] := openRec_ty_subst_ty 0 t σ lc X
+
+/-- Specialize `Term.open_ty_subst` to free type variables. -/
+lemma open_ty_subst_ty_var (t : Term Var) (neq : Y ≠ X) (lc : δ.LC) :
+    (t ^ᵗᵞ .fvar Y)[X := δ] = t[X := δ] ^ᵗᵞ .fvar Y := by grind [open_ty_subst_ty]
+
+omit [HasFresh Var]
+
+/-- Opening a term to a type is equivalent to opening to a free variable and substituting. -/
+lemma openRec_ty_subst_ty_intro (Y : ℕ) (t : Term Var) (nmem : X ∉ t.fv_ty) : 
+  t⟦Y ↝ δ⟧ᵗᵞ = (t⟦Y ↝ Ty.fvar X⟧ᵗᵞ)[X := δ] := by
+  induction t generalizing X δ Y <;> grind [Ty.openRec_subst_intro]
+
+/-- Specialize `Term.openRec_ty_subst_ty_intro` to the first opening. -/
+lemma open_ty_subst_ty_intro (t : Term Var) (δ : Ty Var) (nmem : X ∉ t.fv_ty) : 
+    t ^ᵗᵞ δ = (t ^ᵗᵞ Ty.fvar X)[X := δ] := openRec_ty_subst_ty_intro _ _ nmem
+
+/-- Substitution of a term within a term. -/
+@[scoped grind =]
+def subst_tm (x : Var) (s : Term Var) : Term Var → Term Var
+| bvar x => bvar x
+| fvar y => if y = x then s else fvar y
+| abs σ t₁ => abs σ (subst_tm x s t₁)
+| app t₁ t₂ => app (subst_tm x s t₁) (subst_tm x s t₂)
+| tabs σ t₁ => tabs σ (subst_tm x s t₁)
+| tapp t₁ σ => tapp (subst_tm x s t₁) σ
+| let' t₁ t₂ => let' (subst_tm x s t₁) (subst_tm x s t₂)
+| inl t₁ => inl (subst_tm x s t₁)
+| inr t₁ => inr (subst_tm x s t₁)
+| case t₁ t₂ t₃ => case (subst_tm x s t₁) (subst_tm x s t₂) (subst_tm x s t₃)
+
+instance : HasSubstitution (Term Var) Var (Term Var) where
+  subst t x s := Term.subst_tm x s t
+
+@[scoped grind _=_]
+lemma subst_tm_def : subst_tm (x : Var) (s : Term Var) (t : Term Var) = t[x := s] := by rfl
+
+omit [DecidableEq Var] in
+/-- An opening (term to term) appearing in both sides of an equality of terms can be removed. -/
+lemma openRec_tm_neq_eq (neq : x ≠ y) (eq : t⟦y ↝ s₁⟧ᵗᵗ = t⟦y ↝ s₁⟧ᵗᵗ⟦x ↝ s₂⟧ᵗᵗ) : 
+    t = t⟦x ↝ s₂⟧ᵗᵗ := by
+  induction t generalizing x y <;> grind
+
+omit [DecidableEq Var] in
+/-- Elimination of mixed term and type opening. -/
+lemma openRec_ty_tm_eq (eq : t⟦Y ↝ σ⟧ᵗᵞ = t⟦Y ↝ σ⟧ᵗᵞ⟦x ↝ s⟧ᵗᵗ) : t = t⟦x ↝ s⟧ᵗᵗ := by
+  induction t generalizing x Y <;> grind
+
+variable [HasFresh Var]
+
+/-- A locally closed term is unchanged by term opening. -/
+@[scoped grind]
+lemma openRec_tm_lc (lc : t.LC) : t = t⟦x ↝ s⟧ᵗᵗ := by
+  induction lc generalizing x
+  case let' | case | tabs | abs =>
+    have := fresh_exists <| free_union Var
+    congr <;> grind [openRec_tm_neq_eq, openRec_ty_tm_eq]
+  all_goals grind
+
+variable {t s : Term Var} {δ : Ty Var} {x : Var}
+
+omit [HasFresh Var] in
+/-- Substitution of a free term variable not present in a term leaves it unchanged. -/
+lemma subst_tm_fresh (nmem : x ∉ t.fv_tm) (s : Term Var) : t = t[x := s] := by
+  induction t <;> grind
+
+/-- Substitution of a locally closed term distributes with term opening to a term. -/
+lemma openRec_tm_subst_tm (y : ℕ) (t₁ t₂ : Term Var) (lc : s.LC) (x : Var) :
+    (t₁⟦y ↝ t₂⟧ᵗᵗ)[x := s] = (t₁[x := s])⟦y ↝  t₂[x := s]⟧ᵗᵗ := by
+  induction t₁ generalizing y <;> grind
+
+/-- Specialize `Term.openRec_tm_subst_tm` to the first opening. -/
+lemma open_tm_subst_tm (t₁ t₂ : Term Var) (lc : s.LC) (x : Var) :
+    (t₁ ^ᵗᵗ t₂)[x := s] = (t₁[x := s]) ^ᵗᵗ t₂[x := s] := openRec_tm_subst_tm 0 t₁ t₂ lc x
+
+/-- Specialize `Term.openRec_tm_subst_tm` to free term variables. -/ 
+lemma open_tm_subst_tm_var (t : Term Var) (neq : y ≠ x) (lc : s.LC) :
+     (t ^ᵗᵗ fvar y)[x := s] = (t[x := s]) ^ᵗᵗ fvar y := by grind [open_tm_subst_tm]
+
+/-- Substitution of a locally closed type distributes with term opening to a term. -/
+lemma openRec_tm_subst_ty (y : ℕ) (t₁ t₂ : Term Var) (δ : Ty Var) (X : Var) :
+    (t₁⟦y ↝ t₂⟧ᵗᵗ)[X := δ] = (t₁[X := δ])⟦y ↝  t₂[X := δ]⟧ᵗᵗ := by
+  induction t₁ generalizing y <;> grind
+
+/-- Specialize `Term.openRec_tm_subst_ty` to the first opening -/
+lemma open_tm_subst_ty (t₁ t₂ : Term Var) (δ : Ty Var) (X : Var) :
+    (t₁ ^ᵗᵗ t₂)[X := δ] = (t₁[X := δ]) ^ᵗᵗ t₂[X := δ] := openRec_tm_subst_ty 0 t₁ t₂ δ X
+
+/-- Specialize `Term.open_tm_subst_ty` to free term variables -/
+lemma open_tm_subst_ty_var (t₁ : Term Var) (δ : Ty Var) (X y : Var) :
+    (t₁ ^ᵗᵗ fvar y)[X := δ] = (t₁[X := δ]) ^ᵗᵗ fvar y := by grind [open_tm_subst_ty]
+
+/-- Substitution of a locally closed term distributes with term opening to a type. -/
+lemma openRec_ty_subst_tm (Y : ℕ) (t : Term Var) (δ : Ty Var) (lc : s.LC) (x : Var) :
+    (t⟦Y ↝ δ⟧ᵗᵞ)[x := s] = t[x := s]⟦Y ↝ δ⟧ᵗᵞ := by
+  induction t generalizing Y <;> grind
+
+/-- Specialize `Term.openRec_ty_subst_tm` to the first opening. -/
+lemma open_ty_subst_tm (t : Term Var) (δ : Ty Var) (lc : s.LC) (x : Var) :
+    (t ^ᵗᵞ δ)[x := s] = t[x := s] ^ᵗᵞ δ := openRec_ty_subst_tm 0 t δ lc x
+
+/-- Specialize `Term.open_ty_subst_tm` to free type variables. -/
+lemma open_ty_subst_tm_var (t : Term Var) (lc : s.LC) (x Y : Var) :
+    (t ^ᵗᵞ .fvar Y)[x := s] = t[x := s] ^ᵗᵞ .fvar Y := open_ty_subst_tm _ _ lc _
+
+omit [HasFresh Var]
+
+/-- Opening a term to a term is equivalent to opening to a free variable and substituting. -/
+lemma openRec_tm_subst_tm_intro (y : ℕ) (t s : Term Var) (nmem : x ∉ t.fv_tm) :
+    t⟦y ↝ s⟧ᵗᵗ = (t⟦y ↝ fvar x⟧ᵗᵗ)[x := s] := by
+  induction t generalizing y <;> grind
+
+/-- Specialize `Term.openRec_tm_subst_tm_intro` to the first opening. -/
+lemma open_tm_subst_tm_intro (t s : Term Var) (nmem : x ∉ t.fv_tm) :
+    t ^ᵗᵗs = (t ^ᵗᵗ fvar x)[x := s] := openRec_tm_subst_tm_intro _ _ _ nmem
+
+variable [HasFresh Var]
+
+lemma subst_ty_lc (t_lc : t.LC) (δ_lc : δ.LC) (X : Var) : t[X := δ].LC := by
+  induction t_lc
+  case' abs  => apply LC.abs (free_union Var)
+  case' tabs => apply LC.tabs (free_union Var)
+  case' let' => apply LC.let' (free_union Var)
+  case' case => apply LC.case (free_union Var)
+  all_goals grind [Ty.subst_lc, open_tm_subst_ty_var, openRec_ty_subst_ty]
+
+lemma subst_tm_lc (t_lc : t.LC) (s_lc : s.LC) (x : Var) : t[x := s].LC := by
+  induction t_lc
+  case' abs  => apply LC.abs (free_union Var)
+  case' let' => apply LC.let' (free_union Var)
+  case' case => apply LC.case (free_union Var)
+  case' tabs => apply LC.tabs (free_union Var)
+  all_goals grind [open_tm_subst_tm_var, open_ty_subst_tm_var]
+
+end Term
+
+namespace Binding
+
+omit [HasFresh Var]
+
+/-- Binding substitution of types. -/
+@[scoped grind =]
+def subst (X : Var) (δ : Ty Var) : Binding Var → Binding Var
+| sub γ => sub <| γ[X := δ]
+| ty  γ => ty  <| γ[X := δ]
+
+instance : HasSubstitution (Binding Var) Var (Ty Var) where
+  subst γ X δ := Binding.subst X δ γ
+
+variable {δ γ : Ty Var} {X : Var}
+
+@[scoped grind _=_]
+lemma subst_sub : (sub γ)[X := δ] = sub (γ[X := δ]) := by rfl
+
+@[scoped grind _=_]
+lemma subst_ty : (ty γ)[X := δ] = ty (γ[X := δ]) := by rfl
+
+open scoped Ty in
+/-- Substitution of a free variable not present in a binding leaves it unchanged. -/
+lemma subst_fresh {γ : Binding Var} (nmem : X ∉ γ.fv) (δ : Ty Var) : γ = γ[X := δ] := by
+  induction γ <;> grind [Ty.subst_fresh]
+
+end Binding
+
+end LambdaCalculus.LocallyNameless.Fsub
