Cslib/Languages/LambdaCalculus/LocallyNameless/Fsub/Reduction.lean
@@ -1,0 +1,123 @@
+/-
+Copyright (c) 2025 Chris Henson. All rights reserved.
+Released under Apache 2.0 license as described in the file LICENSE.
+Authors: Chris Henson
+-/
+
+import Cslib.Languages.LambdaCalculus.LocallyNameless.Fsub.Opening
+import Cslib.Foundations.Semantics.ReductionSystem.Basic
+
+/-! # λ-calculus
+
+The λ-calculus with polymorphism and subtyping, with a locally nameless representation of syntax.
+This file defines a call-by-value reduction.
+
+## References
+
+* [A. Chargueraud, *The Locally Nameless Representation*][Chargueraud2012]
+* See also <https://www.cis.upenn.edu/~plclub/popl08-tutorial/code/>, from which
+  this is adapted
+
+-/
+
+variable {Var : Type*}
+
+namespace LambdaCalculus.LocallyNameless.Fsub
+
+namespace Term
+
+/-- Existential predicate for being a locally closed body of an abstraction. -/
+@[scoped grind =]
+def body (t : Term Var) := ∃ L : Finset Var, ∀ x ∉ L, LC (t ^ᵗᵗ fvar x)
+
+section
+
+variable {t₁ t₂ t₃ : Term Var}
+
+variable [DecidableEq Var]
+
+/-- Locally closed let bindings have a locally closed body. -/
+@[scoped grind _=_]
+lemma body_let : (let' t₁ t₂).LC ↔ t₁.LC ∧ t₂.body := by
+  constructor <;> intro h <;> cases h
+  case mp.let' L _ _ =>
+    split_ands
+    · grind
+    · exists L
+  case mpr.intro body =>
+    obtain ⟨_, _⟩ := body
+    apply LC.let' (free_union Var) <;> grind
+
+/-- Locally closed case bindings have a locally closed bodies. -/
+@[scoped grind _=_]
+lemma body_case : (case t₁ t₂ t₃).LC ↔ t₁.LC ∧ t₂.body ∧ t₃.body := by
+  constructor <;> intro h
+  case mp =>
+    cases h with | case L =>
+    split_ands
+    · grind
+    · exists L
+    · exists L
+  case mpr =>
+    obtain ⟨_, ⟨_, _⟩, ⟨_, _⟩⟩ := h
+    apply LC.case (free_union Var) <;> grind
+
+variable [HasFresh Var]
+
+/-- Opening a body preserves local closure. -/
+@[scoped grind <=]
+lemma open_tm_body (body : t₁.body) (lc : t₂.LC) : (t₁ ^ᵗᵗ t₂).LC := by
+  cases body
+  have := fresh_exists <| free_union [fv_tm] Var
+  grind [subst_tm_lc, open_tm_subst_tm_intro]
+
+end
+
+/-- Values are irreducible terms. -/
+@[grind]
+inductive Value : Term Var → Prop
+  | abs : LC (abs σ t₁) → Value (abs σ t₁)
+  | tabs : LC (tabs σ t₁) → Value (tabs σ t₁)
+  | inl : Value t₁ → Value (inl t₁)
+  | inr : Value t₁ → Value (inr t₁)
+
+@[grind →]
+lemma Value.lc {t : Term Var} (val : t.Value) : t.LC := by
+  induction val <;> grind
+
+/-- The call-by-value reduction relation. -/
+@[grind, reduction_sys rs "βᵛ"]
+inductive Red : Term Var → Term Var → Prop
+  | appₗ : LC t₂ → Red t₁ t₁' → Red (app t₁ t₂) (app t₁' t₂)
+  | appᵣ : Value t₁ → Red t₂ t₂' → Red (app t₁ t₂) (app t₁ t₂')
+  | tapp : σ.LC → Red t₁ t₁' → Red (tapp t₁ σ) (tapp t₁' σ)
+  | abs : LC (abs σ t₁) → Value t₂ → Red (app (abs σ t₁) t₂) (t₁ ^ᵗᵗ t₂)
+  | tabs : LC (tabs σ t₁) → τ.LC → Red (tapp (tabs σ t₁) τ) (t₁ ^ᵗᵞ τ)
+  | let_bind : Red t₁ t₁' → t₂.body → Red (let' t₁ t₂) (let' t₁' t₂)
+  | let_body : Value t₁ → t₂.body → Red (let' t₁ t₂) (t₂ ^ᵗᵗ t₁)
+  | inl : Red t₁ t₁' → Red (inl t₁) (inl t₁')
+  | inr : Red t₁ t₁' → Red (inr t₁) (inr t₁')
+  | case : Red t₁ t₁' → t₂.body → t₃.body → Red (case t₁ t₂ t₃) (case t₁' t₂ t₃)
+  | case_inl : Value t₁ → t₂.body → t₃.body → Red (case (inl t₁) t₂ t₃) (t₂ ^ᵗᵗ t₁)
+  | case_inr : Value t₁ → t₂.body → t₃.body → Red (case (inr t₁) t₂ t₃) (t₃ ^ᵗᵗ t₁)
+
+@[grind _=_]
+private lemma rs_eq {t t' : Term Var} : t ⭢βᵛ t' ↔ Red t t' := by
+  have : (@rs Var).Red = Red := by rfl
+  simp_all
+
+variable [HasFresh Var] [DecidableEq Var] in
+/-- Terms of a reduction are locally closed. -/
+lemma Red.lc {t t' : Term Var} (red : t ⭢βᵛ t') : t.LC ∧ t'.LC := by
+  induction red
+  case abs lc _ | tabs lc _ => 
+    split_ands
+    · grind
+    · cases lc
+      have := fresh_exists <| free_union [fv_tm, fv_ty] Var
+      grind [subst_tm_lc, subst_ty_lc, open_tm_subst_tm_intro, open_ty_subst_ty_intro]
+  all_goals grind
+
+end Term
+
+end LambdaCalculus.LocallyNameless.Fsub
