Cslib/Languages/LambdaCalculus/LocallyNameless/Fsub/Safety.lean
@@ -1,0 +1,153 @@
+/-
+Copyright (c) 2025 Chris Henson. All rights reserved.
+Released under Apache 2.0 license as described in the file LICENSE.
+Authors: Chris Henson
+-/
+
+import Cslib.Languages.LambdaCalculus.LocallyNameless.Fsub.Typing
+import Cslib.Languages.LambdaCalculus.LocallyNameless.Fsub.Reduction
+
+/-! # λ-calculus
+
+The λ-calculus with polymorphism and subtyping, with a locally nameless representation of syntax.
+This file proves type safety.
+
+## References
+
+* [A. Chargueraud, *The Locally Nameless Representation*][Chargueraud2012]
+* See also <https://www.cis.upenn.edu/~plclub/popl08-tutorial/code/>, from which
+  this is adapted
+
+-/
+
+variable {Var : Type*} [HasFresh Var] [DecidableEq Var]
+
+namespace LambdaCalculus.LocallyNameless.Fsub
+
+open Context List Env.Wf Term Ty
+
+variable {t : Term Var}
+
+/-- Any reduction step preserves typing. -/
+lemma Typing.preservation (der : Typing Γ t τ) (step : t ⭢βᵛ t') : Typing Γ t' τ := by
+  induction der generalizing t' 
+  case app Γ _ σ τ _ _ _ _ _ => 
+    cases step
+    case appₗ | appᵣ => grind
+    case abs der _ _ =>
+      have sub : Sub Γ (σ.arrow τ) (σ.arrow τ) := by grind [Sub.refl]
+      have ⟨_, _, ⟨_, _⟩⟩ := der.abs_inv sub
+      have ⟨_, _⟩ := fresh_exists <| free_union [fv_tm] Var
+      grind [open_tm_subst_tm_intro, subst_tm, Sub.weaken]
+  case tapp Γ _ σ τ σ' _ _ _ =>
+    cases step
+    case tabs der _ _ =>
+      have sub : Sub Γ (σ.all τ) (σ.all τ) := by grind [Sub.refl]
+      have ⟨_, _, ⟨_, _⟩⟩ := der.tabs_inv sub
+      have ⟨X, _⟩ := fresh_exists <| free_union [Ty.fv, fv_ty] Var
+      have : Γ = (Context.map_val (·[X:=σ']) []) ++ Γ := by simp
+      rw [open_ty_subst_ty_intro (X := X), open_subst_intro (X := X)] <;> grind [subst_ty]
+    case tapp => grind
+  case let' Γ _ _ _ _ L der _ ih₁ _ => 
+    cases step
+    case let_bind red₁ _ => apply Typing.let' L (ih₁ red₁); grind
+    case let_body =>
+      have ⟨x, _⟩ := fresh_exists <| free_union [fv_tm] Var
+      grind [open_tm_subst_tm_intro, subst_tm]
+  case case Γ _ σ τ _ _ _ L _ _ _ ih₁ _ _ => 
+    have sub : Sub Γ (σ.sum τ) (σ.sum τ) := by grind [Sub.refl]
+    have : Γ = [] ++ Γ := by rfl
+    cases step
+    case «case» red₁ _ _ => apply Typing.case L (ih₁ red₁) <;> grind
+    case case_inl der _ _ => 
+      have ⟨_, ⟨_, _⟩⟩ := der.inl_inv sub
+      have ⟨x, _⟩ := fresh_exists <| free_union [fv_tm] Var
+      grind [open_tm_subst_tm_intro, subst_tm]
+    case case_inr der _ _ => 
+      have ⟨_, ⟨_, _⟩⟩ := der.inr_inv sub
+      have ⟨x, _⟩ := fresh_exists <| free_union [fv_tm] Var
+      grind [open_tm_subst_tm_intro, subst_tm]
+  all_goals grind [cases Red]
+
+/-- Any typable term either has a reduction step or is a value. -/
+lemma Typing.progress (der : Typing [] t τ) : t.Value ∨ ∃ t', t ⭢βᵛ t' := by
+  generalize eq : [] = Γ at der
+  have der' : Typing Γ t τ := by assumption
+  induction der <;> subst eq <;> simp only [forall_const] at *
+  case var mem => grind
+  case app t₁ _ _ t₂ l r ih_l ih_r => 
+    right
+    cases ih_l l with
+    | inl val_l => 
+        cases ih_r r with
+        | inl val_r => 
+            have ⟨σ, t₁, eq⟩ := l.canonical_form_abs val_l
+            exists t₁ ^ᵗᵗ t₂
+            grind
+        | inr red_r => 
+            obtain ⟨t₂', _⟩ := red_r
+            exists t₁.app t₂'
+            grind
+    | inr red_l => 
+        obtain ⟨t₁', _⟩ := red_l
+        exists t₁'.app t₂
+        grind
+  case tapp σ' der _ ih => 
+    right
+    specialize ih der
+    cases ih with
+    | inl val => 
+        obtain ⟨_, t, _⟩ := der.canonical_form_tabs val
+        exists t ^ᵗᵞ σ'
+        grind
+    | inr red => 
+        obtain ⟨t', _⟩ := red
+        exists .tapp t' σ'
+        grind
+  case let' t₁ σ t₂ τ L der _ _ ih => 
+    right
+    cases ih der with
+    | inl _ => 
+        exists t₂ ^ᵗᵗ t₁
+        grind
+    | inr red => 
+        obtain ⟨t₁', _⟩ := red
+        exists t₁'.let' t₂
+        grind
+  case inl der _ ih =>
+    cases (ih der) with
+    | inl val => grind
+    | inr red => 
+        right
+        obtain ⟨t', _⟩ := red
+        exists .inl t'
+        grind
+  case inr der _ ih =>
+    cases (ih der) with
+    | inl val => grind
+    | inr red => 
+        right
+        obtain ⟨t', _⟩ := red
+        exists .inr t'
+        grind
+  case case t₁ _ _ t₂ _ t₃ _ der _ _ _ _ ih => 
+    right
+    cases ih der with
+    | inl val => 
+        have ⟨t₁, lr⟩ := der.canonical_form_sum val
+        cases lr <;> [exists t₂ ^ᵗᵗ t₁; exists t₃ ^ᵗᵗ t₁] <;> grind
+    | inr red => 
+        obtain ⟨t₁', _⟩ := red
+        exists t₁'.case t₂ t₃
+        grind
+  case sub => grind
+  case abs σ _ τ L _ _=> 
+    left
+    constructor
+    apply LC.abs L <;> grind [cases Env.Wf, cases Term.LC]
+  case tabs L _ _=>
+    left
+    constructor
+    apply LC.tabs L <;> grind [cases Env.Wf, cases Term.LC]
+
+end LambdaCalculus.LocallyNameless.Fsub
