Cslib/Languages/LambdaCalculus/LocallyNameless/Fsub/Typing.lean
@@ -1,0 +1,241 @@
+/-
+Copyright (c) 2025 Chris Henson. All rights reserved.
+Released under Apache 2.0 license as described in the file LICENSE.
+Authors: Chris Henson
+-/
+
+import Cslib.Languages.LambdaCalculus.LocallyNameless.Fsub.WellFormed
+import Cslib.Languages.LambdaCalculus.LocallyNameless.Fsub.Subtype
+import Cslib.Languages.LambdaCalculus.LocallyNameless.Fsub.Reduction
+
+/-! # λ-calculus
+
+The λ-calculus with polymorphism and subtyping, with a locally nameless representation of syntax.
+This file defines the typing relation.
+
+## References
+
+* [A. Chargueraud, *The Locally Nameless Representation*][Chargueraud2012]
+* See also <https://www.cis.upenn.edu/~plclub/popl08-tutorial/code/>, from which
+  this is adapted
+
+-/
+
+variable {Var : Type*} [DecidableEq Var] [HasFresh Var]
+
+namespace LambdaCalculus.LocallyNameless.Fsub
+
+open Term Ty Ty.Wf Env.Wf Sub Context List Binding
+
+/-- The typing relation. -/
+inductive Typing : Env Var → Term Var → Ty Var → Prop
+  | var : Γ.Wf → Binding.ty σ ∈ Γ.dlookup x → Typing Γ (fvar x) σ
+  | abs (L : Finset Var) :
+      (∀ x ∉ L, Typing (⟨x, Binding.ty σ⟩ :: Γ) (t₁ ^ᵗᵗ fvar x) τ) →
+      Typing Γ (abs σ t₁) (arrow σ τ)
+  | app : Typing Γ t₁ (arrow σ τ) → Typing Γ t₂ σ → Typing Γ (app t₁ t₂) τ
+  | tabs (L : Finset Var) :
+      (∀ X ∉ L, Typing (⟨X, Binding.sub σ⟩ :: Γ) (t₁ ^ᵗᵞ fvar X) (τ ^ᵞ fvar X)) →
+      Typing Γ (tabs σ t₁) (all σ τ)
+  | tapp : Typing Γ t₁ (all σ τ) → Sub Γ σ' σ → Typing Γ (tapp t₁ σ') (τ ^ᵞ σ')
+  | sub : Typing Γ t τ → Sub Γ τ τ' → Typing Γ t τ'
+  | let' (L : Finset Var) :
+      Typing Γ t₁ σ →
+      (∀ x ∉ L, Typing (⟨x, Binding.ty σ⟩ :: Γ) (t₂ ^ᵗᵗ fvar x) τ) →
+      Typing Γ (let' t₁ t₂) τ
+  | inl : Typing Γ t₁ σ → τ.Wf Γ → Typing Γ (inl t₁) (sum σ τ)
+  | inr : Typing Γ t₁ τ → σ.Wf Γ → Typing Γ (inr t₁) (sum σ τ)
+  | case (L : Finset Var) :
+      Typing Γ t₁ (sum σ τ) →
+      (∀ x ∉ L, Typing (⟨x, Binding.ty σ⟩ :: Γ) (t₂ ^ᵗᵗ fvar x) δ) →
+      (∀ x ∉ L, Typing (⟨x, Binding.ty τ⟩ :: Γ) (t₃ ^ᵗᵗ fvar x) δ) →
+      Typing Γ (case t₁ t₂ t₃) δ
+
+namespace Typing
+
+variable {Γ Δ Θ : Env Var} {σ τ δ : Ty Var}
+
+attribute [grind] Typing.var Typing.app Typing.tapp Typing.sub Typing.inl Typing.inr
+
+/-- Typings have well-formed contexts and types. -/
+@[grind →]
+lemma wf {Γ : Env Var} {t : Term Var} {τ : Ty Var} (der : Typing Γ t τ) : Γ.Wf ∧ t.LC ∧ τ.Wf Γ := by
+  induction der <;> let L := free_union Var <;> have := fresh_exists L
+  case tabs => refine ⟨?_, LC.tabs L ?_ ?_, Ty.Wf.all L ?_ ?_⟩ <;> grind [cases Env.Wf]
+  case abs => refine ⟨?_, LC.abs L ?_ ?_, ?_⟩ <;> grind [Wf.strengthen, cases Env.Wf]
+  case let' => refine ⟨?_, LC.let' L ?_ ?_, ?_⟩ <;> grind [Ty.Wf.strengthen]
+  case case => refine ⟨?_, LC.case L ?_ ?_ ?_, ?_⟩ <;> grind [Ty.Wf.strengthen]
+  all_goals grind [of_bind_ty, open_lc, cases Env.Wf, cases Ty.Wf]
+
+/-- Weakening of typings. -/
+lemma weaken (der : Typing (Γ ++ Δ) t τ) (wf : (Γ ++ Θ ++ Δ).Wf) : 
+    Typing (Γ ++ Θ ++ Δ) t τ := by
+  generalize eq : Γ ++ Δ = ΓΔ at der
+  induction der generalizing Γ
+  case' abs => apply abs ((Γ ++ Θ ++ Δ).dom ∪ free_union Var)
+  case' tabs => apply tabs ((Γ ++ Θ ++ Δ).dom ∪ free_union Var)
+  case' let' der _ => apply let' ((Γ ++ Θ ++ Δ).dom ∪ free_union Var) (der wf eq)
+  case' case der _ _ => apply case ((Γ ++ Θ ++ Δ).dom ∪ free_union Var) (der wf eq)
+  all_goals 
+    grind [Wf.weaken, Sub.weaken, Wf.of_env_ty, Wf.of_env_sub, Sub.refl, <= sublist_dlookup]
+
+/-- Weakening of typings (at the front). -/
+lemma weaken_head (der : Typing Δ t τ) (wf : (Γ ++ Δ).Wf) :
+    Typing (Γ ++ Δ) t τ := by
+  have eq : Δ = [] ++ Δ := by rfl
+  rw [eq] at der
+  have := Typing.weaken der wf
+  grind
+
+/-- Narrowing of typings. -/
+lemma narrow (sub : Sub Δ δ δ') (der : Typing (Γ ++ ⟨X, Binding.sub δ'⟩ :: Δ) t τ) :
+    Typing (Γ ++ ⟨X, Binding.sub δ⟩ :: Δ) t τ := by
+  generalize eq : Γ ++ ⟨X, Binding.sub δ'⟩ :: Δ = Θ at der
+  induction der generalizing Γ 
+  case var X' _ _ =>
+    have : X ≠ X' := by grind [→ List.mem_dlookup]
+    have p (δ) : Γ ++ ⟨X, .sub δ⟩ :: Δ ~ ⟨X, .sub δ⟩ :: (Γ ++ Δ) := perm_middle
+    grind [Env.Wf.narrow, List.perm_nodupKeys, => List.perm_dlookup]
+  case' abs  => apply abs (free_union Var)
+  case' tabs => apply tabs (free_union Var)
+  case' let' der _ => apply let' (free_union Var) (der eq)
+  case' case der _ _ => apply case (free_union Var) (der eq)
+  all_goals grind [Ty.Wf.narrow, Env.Wf.narrow, Sub.narrow]
+
+/-- Term substitution within a typing. -/
+lemma subst_tm (der : Typing (Γ ++ ⟨X, .ty σ⟩ :: Δ) t τ) (der_sub : Typing Δ s σ) :
+    Typing (Γ ++ Δ) (t[X := s]) τ := by
+  generalize eq : Γ ++ ⟨X, .ty σ⟩ :: Δ = Θ at der
+  induction der generalizing Γ X
+  case var σ' _ X' _ _ =>
+    have : Γ ++ ⟨X, .ty σ⟩ :: Δ ~ ⟨X, .ty σ⟩ :: (Γ ++ Δ) := perm_middle
+    by_cases eq : X = X'
+    · grind [→ List.mem_dlookup, weaken_head, Env.Wf.strengthen]
+    · grind [Env.Wf.strengthen, => List.perm_dlookup]
+  case abs => 
+    apply abs (free_union Var)
+    grind [open_tm_subst_tm_var]
+  case tabs => 
+    apply tabs (free_union Var)
+    grind [open_ty_subst_tm_var]
+  case let' der _ => 
+    apply let' (free_union Var) (der eq)
+    grind [open_tm_subst_tm_var]
+  case case der _ _ => 
+    apply case (free_union Var) (der eq) <;> grind [open_tm_subst_tm_var]
+  all_goals grind [Env.Wf.strengthen, Ty.Wf.strengthen, Sub.strengthen]
+
+/-- Type substitution within a typing. -/
+lemma subst_ty (der : Typing (Γ ++ ⟨X, Binding.sub δ'⟩ :: Δ) t τ) (sub : Sub Δ δ δ') : 
+    Typing (Γ.map_val (·[X := δ]) ++ Δ) (t[X := δ]) (τ[X := δ]) := by
+  generalize eq : Γ ++ ⟨X, Binding.sub δ'⟩ :: Δ = Θ at der
+  induction der generalizing Γ X 
+  case var σ _ X' _ mem =>
+    have := map_subst_nmem Δ X δ
+    have : Γ ++ ⟨X, .sub δ'⟩ :: Δ ~ ⟨X, .sub δ'⟩ :: (Γ ++ Δ) := perm_middle
+    have : .ty σ ∈ dlookup X' (⟨X, .sub δ'⟩ :: (Γ ++ Δ)) := by grind [perm_dlookup]
+    have := @map_val_mem Var (f := ((·[X:=δ]) : Binding Var → Binding Var))
+    grind [Env.Wf.map_subst, keys_append, → notMem_keys_of_nodupKeys_cons]
+  case abs => 
+    apply abs (free_union [Ty.fv] Var)
+    grind [Ty.subst_fresh, open_tm_subst_ty_var]
+  case tabs => 
+    apply tabs (free_union Var)
+    grind [open_ty_subst_ty_var, open_subst_var]
+  case let' der _ => 
+    apply let' (free_union Var) (der eq)
+    grind [open_tm_subst_ty_var]
+  case case der _ _ =>
+    apply case (free_union Var) (der eq) <;> grind [open_tm_subst_ty_var]
+  case tapp => grind [Ty.open_subst, Env.Wf.map_subst, Ty.Wf.map_subst, Sub.map_subst]
+  all_goals grind [Env.Wf.map_subst, Ty.Wf.map_subst, Sub.map_subst]
+
+open Term Ty
+
+omit [HasFresh Var]
+
+/-- Invert the typing of an abstraction. -/
+lemma abs_inv (der : Typing Γ (.abs γ' t) τ) (sub : Sub Γ τ (arrow γ δ)) :
+     Sub Γ γ γ'
+  ∧ ∃ δ' L, ∀ x ∉ (L : Finset Var), 
+    Typing (⟨x, Binding.ty γ'⟩ :: Γ) (t ^ᵗᵗ .fvar x) δ' ∧ Sub Γ δ' δ := by
+  generalize eq : Term.abs γ' t = e at der
+  induction der generalizing t γ' γ δ
+  case abs τ L _ _ => 
+    cases eq
+    cases sub
+    split_ands
+    · assumption
+    · exists τ, L
+      grind
+  case sub Γ _ τ τ' _ _ ih => 
+    subst eq
+    have sub' : Sub Γ τ (γ.arrow δ) := by grind
+    obtain ⟨_, δ', L, _⟩ := ih sub' (by rfl)
+    split_ands
+    · assumption
+    · exists δ', L
+  all_goals grind
+
+variable [HasFresh Var] in
+/-- Invert the typing of a type abstraction. -/
+lemma tabs_inv (der : Typing Γ (.tabs γ' t) τ) (sub : Sub Γ τ (all γ δ)) :
+     Sub Γ γ γ'
+  ∧ ∃ δ' L, ∀ X ∉ (L : Finset Var),
+     Typing (⟨X, Binding.sub γ⟩ :: Γ) (t ^ᵗᵞ fvar X) (δ' ^ᵞ fvar X)
+     ∧ Sub (⟨X, Binding.sub γ⟩ :: Γ) (δ' ^ᵞ fvar X) (δ ^ᵞ fvar X) := by
+  generalize eq : Term.tabs γ' t = e at der
+  induction der generalizing γ δ t γ'
+  case tabs σ Γ _ τ L der _ =>
+    cases sub with | all L' sub => 
+    split_ands
+    · grind
+    · exists τ, L ∪ L'
+      intro X _
+      have eq : ⟨X, Binding.sub γ⟩ :: Γ = [] ++ ⟨X, Binding.sub γ⟩ :: Γ := by rfl
+      grind [narrow]
+  case sub Γ _ τ τ' _ _ ih => 
+    subst eq
+    have sub' : Sub Γ τ (γ.all δ) := by trans τ' <;> grind
+    obtain ⟨_, δ', L, _⟩ := ih sub' (by rfl)
+    split_ands
+    · assumption
+    · exists δ', L
+  all_goals grind
+
+/-- Invert the typing of a left case. -/
+lemma inl_inv (der : Typing Γ (.inl t) τ) (sub : Sub Γ τ (sum γ δ)) :
+    ∃ γ', Typing Γ t γ' ∧ Sub Γ γ' γ := by
+  generalize eq : t.inl =t at der
+  induction der generalizing γ δ <;> grind [cases Sub]
+
+/-- Invert the typing of a right case. -/
+lemma inr_inv (der : Typing Γ (.inr t) T) (sub : Sub Γ T (sum γ δ)) :
+    ∃ δ', Typing Γ t δ' ∧ Sub Γ δ' δ := by
+  generalize eq : t.inr =t at der
+  induction der generalizing γ δ <;> grind [cases Sub]
+
+/-- A value that types as a function is an abstraction. -/
+lemma canonical_form_abs (val : Value t) (der : Typing [] t (arrow σ τ)) :
+    ∃ δ t', t = .abs δ t' := by
+  generalize eq  : σ.arrow τ = γ at der
+  generalize eq' : [] = Γ at der
+  induction der generalizing σ τ <;> grind [cases Sub, cases Value]
+
+/-- A value that types as a quantifier is a type abstraction. -/
+lemma canonical_form_tabs (val : Value t) (der : Typing [] t (all σ τ)) :
+    ∃ δ t', t = .tabs δ t' := by
+  generalize eq  : σ.all τ = γ at der
+  generalize eq' : [] = Γ at der
+  induction der generalizing σ τ <;> grind [cases Sub, cases Value]
+
+/-- A value that types as a sum is a left or right case. -/
+lemma canonical_form_sum (val : Value t) (der : Typing [] t (sum σ τ)) :
+    ∃ t', t = .inl t' ∨ t = .inr t' := by
+  generalize eq  : σ.sum τ = γ at der
+  generalize eq' : [] = Γ at der
+  induction der generalizing σ τ <;> grind [cases Sub, cases Value]
+
+end Typing
+
+end LambdaCalculus.LocallyNameless.Fsub
